Verificacion de algoritmo 2-Aproximado

Algoritmos Aproximados/Envasado.dfy/Envasado2Aproximado.dfy
@@ -8,10 +8,11 @@ lemma ValidCapacity(bins: seq<multiset<nat>>, bins': seq<multiset<nat>>, capacit
 requires 0 <= idx < |bins|
 requires |bins| == |capacity|
 requires capacity[idx] + currElement <= E
-requires forall i: nat | 0 <= i < |bins| :: GSumNat(bins[i]) == capacity[i] && capacity[i] <= E
+requires forall i: nat | 0 <= i < |bins| :: GSumNat(bins[i]) == capacity[i] && 0 < capacity[i] <= E
 requires bins' == bins[idx := (bins[idx] + multiset{currElement})]
 requires capacity' == capacity[idx := capacity[idx] + currElement]
-ensures forall i: nat | 0 <= i < |bins'| :: GSumNat(bins'[i]) == capacity'[i] && capacity'[i] <= E
+requires currElement > 0
+ensures forall i: nat | 0 <= i < |bins'| :: GSumNat(bins'[i]) == capacity'[i] && 0 < capacity'[i] <= E
 {
     GSumIntElemIn(bins'[idx], currElement);
     assert bins'[idx] - multiset{currElement} == bins[idx];
@@ -22,13 +23,343 @@ ensures forall i: nat | 0 <= i < |bins'| :: GSumNat(bins'[i]) == capacity'[i] &&
 //After putting currElement in bin i, the capacities of all packs is still valid
 lemma ValidCapacityNotFit(bins: seq<multiset<nat>>, bins': seq<multiset<nat>>, capacity: seq<nat>, capacity': seq<nat>, E: nat, currElement: nat)
 requires |bins| == |capacity|
-requires currElement <= E
-requires forall i: nat | 0 <= i < |bins| :: GSumNat(bins[i]) == capacity[i] && capacity[i] <= E
+requires 0 < currElement <= E
+requires forall i: nat | 0 <= i < |bins| :: GSumNat(bins[i]) == capacity[i] && 0 < capacity[i] <= E
 requires bins' == bins + [multiset{currElement}]
 requires capacity' == capacity + [currElement]
-ensures forall i: nat | 0 <= i < |bins'| :: GSumNat(bins'[i]) == capacity'[i] && capacity'[i] <= E
+ensures forall i: nat | 0 <= i < |bins'| :: GSumNat(bins'[i]) == capacity'[i] && 0 < capacity'[i] <= E
 { }
 
+//If the current element fit in one of the existing bins, it holds that the set of elements in the partial solution and the set of analyzed elements are the same
+lemma PartialSolutionIsAnalyzedFit(bins: seq<multiset<nat>>, bins': seq<multiset<nat>>, currElement: nat, idx: nat, 
+                                   A: multiset<nat>, iterateMultiset: multiset<nat>, iterateMultiset': multiset<nat>)
+requires currElement in iterateMultiset
+requires iterateMultiset' <= A 
+requires iterateMultiset <= A
+requires 0 <= idx < |bins|
+requires iterateMultiset' == iterateMultiset - multiset{currElement}
+requires bins' == bins[idx := (bins[idx] + multiset{currElement})]
+requires Union(multiset(bins)) == A - iterateMultiset
+ensures Union(multiset(bins')) == A - iterateMultiset'
+{
+    var I: multiset<multiset<nat>> := multiset(bins);
+    var I': multiset<multiset<nat>> := I - multiset{bins[idx]};
+    var I'': multiset<multiset<nat>> := I' + multiset{bins[idx] + multiset{currElement}};
+    var analyzed := A - iterateMultiset;
+    var analyzed' := A - iterateMultiset';
+    
+    calc{
+        Union(multiset(bins'));
+        {assert multiset(bins') == I'';}
+        Union(I'');
+        {
+            UnionOne(I'', bins'[idx]);
+            assert I'' - multiset{bins'[idx]} == I';
+        }
+        Union(I') + bins'[idx];
+        {UnionOne(I, bins[idx]);}
+        Union(I) - bins[idx] + bins'[idx];
+        analyzed - bins[idx] + bins'[idx];
+        {
+            //assert bins[idx] in I;
+            UnionOne(I, bins[idx]);
+            //assert bins[idx] <= Union(I);
+            SubMultisetUnionDifference(analyzed, bins[idx], bins'[idx]);
+        }
+        analyzed + multiset{currElement};
+        A - iterateMultiset + multiset{currElement};
+        {DifferenceOfDifference(A, iterateMultiset', iterateMultiset, currElement);}
+        A - iterateMultiset';
+    }
+}
+
+lemma PartialSolutionIsAnalyzedNotFit(bins: seq<multiset<nat>>, bins': seq<multiset<nat>>, currElement: nat, 
+                                      A: multiset<nat>, iterateMultiset: multiset<nat>, iterateMultiset': multiset<nat>)
+requires bins' == bins + [multiset{currElement}]
+requires currElement in iterateMultiset
+requires iterateMultiset' <= A 
+requires iterateMultiset <= A
+requires iterateMultiset' == iterateMultiset - multiset{currElement}
+requires Union(multiset(bins)) == A - iterateMultiset
+ensures A - iterateMultiset' == Union(multiset(bins'))
+{ 
+    var analyzed := A - iterateMultiset;
+    calc{
+        Union(multiset(bins'));
+        { UnionOne(multiset(bins'), multiset{currElement}); }
+        multiset{currElement} + Union(multiset(bins') - multiset{multiset{currElement}});
+        { assert multiset(bins) == multiset(bins') - multiset{multiset{currElement}}; }
+        multiset{currElement} + Union(multiset(bins));
+        multiset{currElement} + analyzed;
+        analyzed + multiset{currElement};
+        A - iterateMultiset + multiset{currElement};
+        {DifferenceOfDifference(A, iterateMultiset', iterateMultiset, currElement);}
+        A - iterateMultiset';
+    }
+}
+
+//After adding the current element to an existing bin, each bin is still a subset of analyzed
+lemma SubmultisetIfFit(bins: seq<multiset<nat>>, bins': seq<multiset<nat>>, currElement: nat, idx: nat, A: multiset<nat>, iterateMultiset: multiset<nat>, iterateMultiset': multiset<nat>)
+requires 0 <= idx < |bins|
+requires bins' == bins[idx := (bins[idx] + multiset{currElement})]
+requires forall i: nat | 0 <= i < |bins| :: bins[i] <= A-iterateMultiset
+requires iterateMultiset <= A
+requires iterateMultiset' <= A
+requires currElement in iterateMultiset 
+requires iterateMultiset' == iterateMultiset - multiset{currElement}
+ensures forall i: nat | 0 <= i < |bins'| :: bins'[i] <= A-iterateMultiset'
+{ 
+    calc{
+        A - iterateMultiset';
+        A - (iterateMultiset - multiset{currElement});
+        {DifferenceOfDifference(A, iterateMultiset', iterateMultiset, currElement);}
+        A - iterateMultiset + multiset{currElement};
+    }
+}
+
+//After adding the current element to an existing bin, each bin is still a subset of analyzed
+lemma SubmultisetIfNotFit(bins: seq<multiset<nat>>, bins': seq<multiset<nat>>, currElement: nat, A: multiset<nat>, iterateMultiset: multiset<nat>, iterateMultiset': multiset<nat>)
+requires bins' == bins + [multiset{currElement}]
+requires forall i: nat | 0 <= i < |bins| :: bins[i] <= A-iterateMultiset
+requires iterateMultiset <= A
+requires iterateMultiset' <= A
+requires currElement in iterateMultiset 
+requires iterateMultiset' == iterateMultiset - multiset{currElement}
+ensures forall i: nat | 0 <= i < |bins'| :: bins'[i] <= A-iterateMultiset'
+{ 
+    calc{
+        A - iterateMultiset';
+        A - (iterateMultiset - multiset{currElement});
+        {DifferenceOfDifference(A, iterateMultiset', iterateMultiset, currElement);}
+        A - iterateMultiset + multiset{currElement};
+    }
+}
+
+//If the current element could not fit in an of the existing bins, after creating a new bin to put it in, at most one bin is half or less full
+lemma AtMostOneLessThanHalfFullNotFit(bins: seq<multiset<nat>>, bins': seq<multiset<nat>>, currElement: nat, E: nat)
+requires bins' == bins + [multiset{currElement}]
+requires currElement <= E
+requires allMoreThanHalfFullSeq(E, bins) || oneLessThanHalfFullSeq(E, bins)
+requires forall i: nat | 0 <= i < |bins| :: GSumNat(bins[i]) + currElement > E
+ensures allMoreThanHalfFullSeq(E, bins') || oneLessThanHalfFullSeq(E, bins')
+{ }
+
+//If the current element could not fit in an of the existing bins, after creating a new bin to put it in, at most one bin is half or less full
+lemma AtMostOneLessThanHalfFullFit(E: nat, bins: seq<multiset<nat>>, bins': seq<multiset<nat>>, idx: nat, currElement: nat)
+requires 0 <= idx < |bins|
+requires bins' == bins[idx := (bins[idx] + multiset{currElement})]
+requires forall i: nat | 0 <= i < |bins'| :: GSumNat(bins'[i]) <= E
+requires forall i: nat | 0 <= i < |bins| :: GSumNat(bins[i]) <= E
+requires allMoreThanHalfFullSeq(E, bins) || oneLessThanHalfFullSeq(E, bins)
+ensures allMoreThanHalfFullSeq(E, bins') || oneLessThanHalfFullSeq(E, bins')
+{
+    if currElement * 2 > E {
+        if allMoreThanHalfFullSeq(E, bins){
+            assert GSumNat(bins[idx]) * 2 > E; 
+            assert currElement * 2 > E;
+            assert currElement + GSumNat(bins[idx]) > E;
+            GSumIntElemIn(bins'[idx], currElement);
+            calc{
+                GSumNat(bins'[idx]);
+                {GSumPositiveIntNat(bins'[idx]);}
+                GSumInt(bins'[idx]);
+                {GSumIntElemIn(bins'[idx], currElement);}
+                currElement + GSumInt(bins'[idx] - multiset{currElement});
+                {
+                    GSumPositiveIntNat(bins[idx]);
+                    assert bins'[idx] - multiset{currElement} == bins[idx];   
+                }
+                currElement + GSumNat(bins[idx]);
+            }
+            assert GSumNat(bins'[idx]) > E;
+            assert false;
+        }
+        else{  
+            var lessThanHalf: nat :| 0 <= lessThanHalf < |bins| && GSumNat(bins[lessThanHalf]) * 2 <= E && 
+                    forall lessThanHalf': nat | 0 <= lessThanHalf' < |bins| && lessThanHalf' != lessThanHalf :: GSumNat(bins[lessThanHalf']) * 2 > E;
+            assert lessThanHalf == idx by
+            {
+                if lessThanHalf != idx {
+                    GSumIntElemIn(bins'[idx], currElement);
+                    assert bins'[idx] - multiset{currElement} == bins[idx];
+                    GSumPositiveIntNat(bins'[idx]);
+                    GSumPositiveIntNat(bins[idx]);
+                }
+            }
+        }
+    }
+    else{ 
+        if allMoreThanHalfFullSeq(E, bins){}
+        else{
+            var lessThanHalf: nat :| 0 <= lessThanHalf < |bins| && GSumNat(bins[lessThanHalf]) * 2 <= E && 
+                    forall lessThanHalf': nat | 0 <= lessThanHalf' < |bins| && lessThanHalf' != lessThanHalf :: GSumNat(bins[lessThanHalf']) * 2 > E;
+            if lessThanHalf == idx {}
+            else{
+                GSumPositiveIntNat(bins[idx]);
+                GSumIntElemIn(bins'[idx], currElement);
+                assert bins'[idx] - multiset{currElement} == bins[idx];
+                GSumPositiveIntNat(bins'[idx]);
+            }
+        }
+     }
+}
+
+//Preducate that gorups all the invariants held by the loop
+ghost predicate invariantLoop(A: multiset<nat>, E: nat, bins:seq<multiset<nat>>, capacity: seq<nat>, iterateMultiset:multiset<nat>)
+{ 
+    0 <= |bins| == |capacity| &&
+    iterateMultiset <= A &&
+    (forall i: nat | 0 <= i < |bins| :: bins[i] <= A && GSumNat(bins[i]) == capacity[i] && 0 < capacity[i] <= E) &&
+    A-iterateMultiset == Union(multiset(bins)) &&
+    (forall i: nat | 0 <= i < |bins| :: bins[i] <= A - iterateMultiset) &&
+    (allMoreThanHalfFullSeq(E, bins) || oneLessThanHalfFullSeq(E, bins))
+}
+
+//This does verify, but it takes a couple of minutes            
+method binPacking2AproximatedGeneralBodyLoop(A: multiset<nat>, E: nat,bins:seq<multiset<nat>>, capacity: seq<nat>,iterateMultiset:multiset<nat>) returns (newbins:seq<multiset<nat>>, newcapacity: seq<nat>, newiterateMultiset:multiset<nat>)
+requires forall a: nat | a in A :: 0 < a <= E
+requires invariantLoop(A,E,bins,capacity,iterateMultiset)
+requires iterateMultiset != multiset{}
+ensures invariantLoop(A,E,newbins,newcapacity,newiterateMultiset)
+ensures newiterateMultiset < iterateMultiset
+{       
+    //assume false;
+    var j := 0;
+    var currElement: nat := pickMultiset(iterateMultiset);
+
+    while j < |bins| && capacity[j] + currElement > E
+    decreases |bins|-j
+    invariant 0 <= j <= |bins| 
+    invariant forall k | 0 <= k < j :: capacity[k] + currElement > E
+    { 
+        j:= j+1;
+    }
+    //These invariants do not need proof to verify
+    //Current element did not fit in any of the existing bins
+    if (j == |bins|) {
+        newbins := bins + [multiset{currElement}];
+        newcapacity := capacity + [currElement];
+        newiterateMultiset := iterateMultiset - multiset{currElement};
+
+        //Proof for (forall i: nat | 0 <= i < |bins| :: bins[i] <= A && GSumNat(bins[i]) == capacity[i] && capacity[i] <= E)
+        ValidCapacityNotFit(bins, newbins, capacity, newcapacity, E, currElement);
+        //Proof for A-iterateMultiset == Union(multiset(bins)) 
+        PartialSolutionIsAnalyzedNotFit(bins, newbins, currElement, A, iterateMultiset, newiterateMultiset);
+        //Proof for forall i: nat | 0 <= i < |bins| :: bins[i] <= A - iterateMultiset 
+        SubmultisetIfNotFit(bins, newbins, currElement, A, iterateMultiset, newiterateMultiset);
+        //assert forall i: nat | 0 <= i < |newbins| :: newbins[i] <= A-newiterateMultiset;
+        //assume false;
+        //Proof for (allMoreThanHalfFullSeq(E, bins) || oneLessThanHalfFullSeq(E, bins))
+        assert newbins == bins + [multiset{currElement}];
+        assert currElement <= E;
+        assert allMoreThanHalfFullSeq(E, bins) || oneLessThanHalfFullSeq(E, bins);
+        assert forall i: nat | 0 <= i < |bins| :: GSumNat(bins[i]) + currElement > E;
+        AtMostOneLessThanHalfFullNotFit(bins, newbins, currElement, E);   
+        //Termination function does decrease
+        assert newiterateMultiset < iterateMultiset;
+    }
+    //Current element did fit in an existing bin
+    else {
+        //assume false;
+        newbins := bins[j := (bins[j] + multiset{currElement})];
+        newcapacity := capacity[j := capacity[j] + currElement];
+        newiterateMultiset := iterateMultiset - multiset{currElement};
+
+        //Lemmas to prove invariants
+        //Proof for valid capacities after putting currElement in pack i
+        ValidCapacity(bins, newbins, capacity, newcapacity, E, currElement, j);
+        //Proof for A-iterateMultiset == Union(multiset(bins))
+        PartialSolutionIsAnalyzedFit(bins, newbins, currElement, j, A, iterateMultiset, newiterateMultiset);
+        //Proof for forall i: nat | 0 <= i < |bins| :: bins[i] <= A - iterateMultiset 
+        SubmultisetIfFit(bins, newbins, currElement, j, A, iterateMultiset, newiterateMultiset);
+        //Proof for (allMoreThanHalfFullSeq(E, bins) || oneLessThanHalfFullSeq(E, bins))
+        AtMostOneLessThanHalfFullFit(E, bins, newbins, j, currElement);  
+        //Termination function does decrease
+        assert newiterateMultiset < iterateMultiset;
+    }
+}
+
+//We use the first fit strategy and check the elements in any order
+//At most only one bin is less than half full, thus we use most twice as many as in the optimal solution
+method binPacking2AproximatedGeneral(A: multiset<nat>, E: nat) returns (I: multiset<multiset<nat>>)
+requires forall a: nat | a in A :: 0 < a <= E
+requires E > 0
+ensures isEnvasado(A,E,I)
+ensures isKAproximatedBinPacking(A, E, I, 2)
+{
+    //Variable initialization
+    //bins will hold the solution, expressed as a multiset of tupples that each represent a bin, in which the first element is the its contents and the second is its capacity
+    var bins: seq<multiset<nat>> := [];
+    var capacity: seq<nat> := [];
+    //iterateMultiset exists to let us iterate over all the elements in A, one by one
+    var iterateMultiset: multiset<nat> := A;
+
+    while iterateMultiset != multiset{}
+    decreases iterateMultiset
+    invariant invariantLoop(A,E,bins,capacity,iterateMultiset)
+    //invariant allMoreThanHalfFull(E, multiset(bins)) || oneLessThanHalfFull(E, multiset(bins))
+    //at most  one bin is less than half full
+    {
+        bins,capacity,iterateMultiset := binPacking2AproximatedGeneralBodyLoop(A,E,bins,capacity,iterateMultiset);
+    }
+    //As the sequence verifies all the coditions necessary to be a BinPacking, so does the corresponding multiset
+    I := multiset(bins);
+    HalfSeqToMultisetTranslation(E, bins);
+    atMostOneLessThanHalfImplies2Aproximated(A, E, I);
+}
+
+/*Version vieja
+
+//When adding a new bin, the partial solution is still a BinPacking over the analyzed nodes
+lemma EnvasadoIfNotFit(I: multiset<multiset<nat>>, I': multiset<multiset<nat>>, currElement: nat, analyzed: multiset<nat>, analyzed': multiset<nat>, E: nat)
+requires I' == I + multiset{multiset{currElement}} 
+requires analyzed' == analyzed + multiset{currElement}
+requires isEnvasado(analyzed, E, I)
+requires currElement <= E
+ensures isEnvasado(analyzed', E, I')
+{ 
+    UnionOne(I', multiset{currElement});
+    assert I' - multiset{multiset{currElement}} == I;
+    assert Union(I') == analyzed';
+}
+
+//If the element was not included in an existing bin the partial solution is still represented by the sequence
+lemma ElementIncludedIfDidNotFits(bins: seq<multiset<nat>>, bins': seq<multiset<nat>>, I: multiset<multiset<nat>>, I': multiset<multiset<nat>>, currElement: nat)
+requires bins' == bins + [multiset{currElement}]
+requires I == multiset(bins)
+requires I' == I + multiset{multiset{currElement}}
+ensures I' == multiset(bins')
+{
+    SequenceCompositionToMultiset(bins, multiset{currElement});
+}
+
+//When the current element fits in an existing bin, the partial solution remains a BinPacking over analyzed
+lemma EnvasadoIfFit(analyzed: multiset<nat>, E: nat, I: multiset<multiset<nat>>, I': multiset<multiset<nat>>, I'': multiset<multiset<nat>>, 
+                    bins: seq<multiset<nat>>, bins': seq<multiset<nat>>, idx: nat, currElement: nat)
+requires 0 <= idx < |bins|
+requires bins' == bins[idx := (bins[idx] + multiset{currElement})]
+requires I == multiset(bins)
+requires I' == I - multiset{bins[idx]}
+requires I'' == I' + multiset{bins'[idx]}
+requires Union(I) == analyzed
+requires isEnvasado(analyzed, E, I)
+requires Union(I'') == analyzed + multiset{currElement}
+requires forall i: nat | 0 <= i < |bins'| :: bins'[i] <= analyzed + multiset{currElement}
+requires forall i: nat | 0 <= i < |bins'| :: GSumNat(bins'[i]) <= E
+ensures isEnvasado(analyzed + multiset{currElement}, E, I'')
+{ }
+
+/*
+//The partition of A is maintained after moving an element from iterateMultiset to analyzed
+lemma partitionMaintained(A: multiset<nat>, iterateMultiset: multiset<nat>, iterateMultiset': multiset<nat>, analyzed: multiset<nat>, analyzed': multiset<nat>, currElement: nat)
+requires A == iterateMultiset + analyzed
+requires currElement in iterateMultiset
+requires iterateMultiset' == iterateMultiset - multiset{currElement}
+requires analyzed' == analyzed + multiset{currElement}
+ensures A == iterateMultiset' + analyzed'
+{ }*/
+
+/*
 //If the element was included in an existing bin the partial solution is still represented by the sequence
 lemma ElementIncludedIfFits(bins: seq<multiset<nat>>, bins': seq<multiset<nat>>, I: multiset<multiset<nat>>, I': multiset<multiset<nat>>, I'': multiset<multiset<nat>>, currElement: nat, idx: nat)
 requires 0 <= idx < |bins|
@@ -45,18 +376,9 @@ ensures I'' == multiset(bins')
         multiset(bins) - multiset{bins[idx]} + multiset{bins'[idx]};
         multiset(bins');
     }
-}
+}*/
 
-//If the element was not included in an existing bin the partial solution is still represented by the sequence
-lemma ElementIncludedIfDidNotFits(bins: seq<multiset<nat>>, bins': seq<multiset<nat>>, I: multiset<multiset<nat>>, I': multiset<multiset<nat>>, currElement: nat)
-requires bins' == bins + [multiset{currElement}]
-requires I == multiset(bins)
-requires I' == I + multiset{multiset{currElement}}
-ensures I' == multiset(bins')
-{
-    SequenceCompositionToMultiset(bins, multiset{currElement});
-}
-
+/*
 //If the current element fit in one of the existing bins, it holds that the set of elements in the partial solution and the set of analyzed elements are the same
 lemma PartialSolutionIsAnalyzedFit(bins: seq<multiset<nat>>, bins': seq<multiset<nat>>, I: multiset<multiset<nat>>, I': multiset<multiset<nat>>, I'': multiset<multiset<nat>>, currElement: nat, idx: nat, analyzed: multiset<nat>)
 requires 0 <= idx < |bins|
@@ -86,37 +408,10 @@ ensures Union(I'') == analyzed + multiset{currElement}
         }
         analyzed + multiset{currElement};
     }
-}
+}*/
 
-//If the current element did not fit in one of the existing bins, it holds that the set of elements in the partial solution and the set of analyzed elements are the same
-lemma PartialSolutionIsAnalyzedNotFit(bins: seq<multiset<nat>>, bins': seq<multiset<nat>>, I: multiset<multiset<nat>>, I': multiset<multiset<nat>>, currElement: nat, analyzed: multiset<nat>)
-requires bins' == bins + [multiset{currElement}]
-requires I == multiset(bins)
-requires I' == I + multiset{multiset{currElement}}
-requires Union(I) == analyzed
-{ }
-
-//The partition of A is maintained after moving an element from iterateMultiset to analyzed
-lemma partitionMaintained(A: multiset<nat>, iterateMultiset: multiset<nat>, iterateMultiset': multiset<nat>, analyzed: multiset<nat>, analyzed': multiset<nat>, currElement: nat)
-requires A == iterateMultiset + analyzed
-requires currElement in iterateMultiset
-requires iterateMultiset' == iterateMultiset - multiset{currElement}
-requires analyzed' == analyzed + multiset{currElement}
-ensures A == iterateMultiset' + analyzed'
-{ }
-
-lemma EnvasadoIfNotFit(I: multiset<multiset<nat>>, I': multiset<multiset<nat>>, currElement: nat, analyzed: multiset<nat>, analyzed': multiset<nat>, E: nat)
-requires I' == I + multiset{multiset{currElement}} 
-requires analyzed' == analyzed + multiset{currElement}
-requires isEnvasado(analyzed, E, I)
-requires currElement <= E
-ensures isEnvasado(analyzed', E, I')
-{ 
-    UnionOne(I', multiset{currElement});
-    assert I' - multiset{multiset{currElement}} == I;
-    assert Union(I') == analyzed';
-}
-
+//After adding the current element to an existing bin, each bin is still a subset of analyzed
+/*
 lemma SubmultisetIfFit(bins: seq<multiset<nat>>, bins': seq<multiset<nat>>, I: multiset<multiset<nat>>, I': multiset<multiset<nat>>, I'': multiset<multiset<nat>>, currElement: nat, idx: nat, analyzed: multiset<nat>)
 requires 0 <= idx < |bins|
 requires bins' == bins[idx := (bins[idx] + multiset{currElement})]
@@ -125,11 +420,14 @@ requires I' == I - multiset{bins[idx]}
 requires I'' == I' + multiset{bins'[idx]}
 requires forall i: nat | 0 <= i < |bins| :: bins[i] <= analyzed 
 ensures forall i: nat | 0 <= i < |bins'| :: bins'[i] <= analyzed + multiset{currElement} 
-{ }
+{ }*/
 
-method bodyLoop(A: multiset<nat>, E: nat, i: nat, bins: seq<multiset<nat>>, capacity: seq<nat>, I: multiset<multiset<nat>>,
+
+/*
+method{:only} bodyLoop(A: multiset<nat>, E: nat, i: nat, bins: seq<multiset<nat>>, capacity: seq<nat>, I: multiset<multiset<nat>>,
                 iterateMultiset:multiset<nat>, analyzed: multiset<nat>, fit: bool, currElement: nat) 
                 returns (rI: multiset<multiset<nat>>, rbins: seq<multiset<nat>>, rcapacity: seq<nat>, rfit: bool, ri: nat)
+requires 0 <= i < |bins|
 requires |bins| == |capacity|
 requires iterateMultiset <= A 
 requires analyzed <= A 
@@ -141,7 +439,10 @@ requires I == multiset(bins)
 requires !fit ==> Union(I) == analyzed
 requires fit ==> Union(I) == analyzed + multiset{currElement}
 requires !fit && 0 <= i < |bins|
-ensures ri >= 0
+requires !fit ==> isEnvasado(analyzed, E, I)
+requires !fit ==> forall idx: nat | 0 <= idx < i :: GSumNat(bins[idx]) + currElement > E
+requires allMoreThanHalfFullSeq(E, bins) || oneLessThanHalfFullSeq(E, bins)
+ensures |rbins| >= ri >= 0
 ensures |rbins| == |rcapacity|
 ensures iterateMultiset <= A 
 ensures analyzed <= A 
@@ -153,9 +454,12 @@ ensures rI == multiset(rbins)
 ensures !rfit ==> Union(rI) == analyzed
 ensures rfit ==> Union(rI) == analyzed + multiset{currElement}
 ensures |bins| - i > |rbins| - ri 
+ensures !rfit ==> isEnvasado(analyzed, E, rI)
+ensures rfit ==> isEnvasado(analyzed + multiset{currElement}, E, rI)
+ensures !rfit ==> forall idx: nat | 0 <= idx < ri :: GSumNat(rbins[idx]) + currElement > E
+//ensures allMoreThanHalfFullSeq(E, rbins) || oneLessThanHalfFullSeq(E, rbins)
 {
-    //assume false;
-    if capacity[i] + currElement < E {
+    if capacity[i] + currElement <= E {
         //Create copy of capacity[i]
         var capacityBefore := capacity[i]; 
 
@@ -175,6 +479,15 @@ ensures |bins| - i > |rbins| - ri
         //Proof for forall i: nat | 0 <= i < |bins| :: bins[i] <= analyzed
         assert forall i: nat | 0 <= i < |bins| :: bins[i] <= analyzed;
         SubmultisetIfFit(bins, bins', I, I', I'', currElement, i, analyzed);
+        //Proof for rfit ==> isEnvasado(analyzed + multiset{currElement}, E, rI)
+        EnvasadoIfFit(analyzed, E, I, I', I'', bins, bins', i, currElement);
+        //Proof for allMoreThanHalfFull(E, rI) || oneLessThanHalfFull(E, rI)requires 0 <= idx < |bins|
+        assert bins' == bins[i := (bins[i] + multiset{currElement})];
+        assert forall i: nat | 0 <= i < |bins'| :: GSumNat(bins'[i]) <= E;
+        assert forall i: nat | 0 <= i < |bins| :: GSumNat(bins[i]) <= E;
+        assert allMoreThanHalfFullSeq(E, bins) || oneLessThanHalfFullSeq(E, bins);
+        assume false;
+        AtMostOneLessThanHalfFullFIt(E, bins, bins', i, currElement);
 
         
         //Update I and bins
@@ -190,6 +503,9 @@ ensures |bins| - i > |rbins| - ri
         rfit := true;
     }
     else{
+        //Proof for !rfit ==> forall idx: nat | 0 <= idx < ri :: GSumNat(rbins[idx]) + currElement > E
+        assert forall idx: nat | 0 <= idx < i :: GSumNat(bins[idx]) + currElement > E;
+
         rI := I;
         rbins := bins;
         rcapacity := capacity;
@@ -202,6 +518,8 @@ ensures |bins| - i > |rbins| - ri
 
 //We use the first fit strategy and check the elements in any order
 //At most only one bin is less than half full, thus we use most twice as many as in the optimal solution
+//falta la otra mitad de AtMostOneLessThanFull, un par de desarrollos para las precodiciones de la llamada AtMostOneLessThanHalfFullNotFIt 
+//y la parte del desarrollo final
 method binPacking2AproximatedGeneral(A: multiset<nat>, E: nat) returns (I: multiset<multiset<nat>>)
 requires forall a: nat | a in A :: 0 < a <= E
 requires E > 0
@@ -225,28 +543,58 @@ ensures isKAproximatedBinPacking(A, E, I, 2)
     invariant forall i: nat | 0 <= i < |bins| :: GSumNat(bins[i]) == capacity[i] && capacity[i] <= E
     invariant isEnvasado(analyzed, E, I)
     invariant I == multiset(bins)
-    //invariant allMoreThanHalfFull(E, I) || oneLessThanHalfFull(E, I)
+    invariant allMoreThanHalfFull(E, I) || oneLessThanHalfFull(E, I)
     //at most  one bin is less than half full
     {
         
         var currElement: nat := pickMultiset(iterateMultiset);
         var i := 0;
         var fit: bool := false;
-
+        //assume false;
+        //
         while !fit && i < |bins|
+        invariant 0 <= i <= |bins|
         invariant |bins| == |capacity|
         invariant iterateMultiset <= A 
+        //
         invariant analyzed <= A 
+        //
         invariant iterateMultiset + analyzed == A
         invariant forall i: nat | 0 <= i < |bins| :: GSumNat(bins[i]) == capacity[i] && capacity[i] <= E
+        //
         invariant !fit ==> forall i: nat | 0 <= i < |bins| :: bins[i] <= analyzed 
         invariant fit ==> forall i: nat | 0 <= i < |bins| :: bins[i] <= analyzed + multiset{currElement}
         invariant I == multiset(bins)
+        //
         invariant !fit ==> Union(I) == analyzed
         invariant fit ==> Union(I) == analyzed + multiset{currElement}
+        //
+        invariant !fit ==> isEnvasado(analyzed, E, I)
+        invariant fit ==> isEnvasado(analyzed + multiset{currElement}, E, I)   
+        //
+        invariant !fit ==> forall idx: nat | 0 <= idx < i :: GSumNat(bins[idx]) + currElement > E
+        //invariant allMoreThanHalfFullSeq(E, bins) || oneLessThanHalfFullSeq(E, bins)
         { 
+            /*
+            assert |bins| == |capacity|;
+            assume false;
+            assert iterateMultiset <= A; 
+            assert analyzed <= A; 
+            assert iterateMultiset + analyzed == A;
+            assert forall i: nat | 0 <= i < |bins| :: GSumNat(bins[i]) == capacity[i] && capacity[i] <= E;
+            assert !fit ==> forall i: nat | 0 <= i < |bins| :: bins[i] <= analyzed; 
+            assert fit ==> forall i: nat | 0 <= i < |bins| :: bins[i] <= analyzed + multiset{currElement};
+            assert I == multiset(bins);
+            assert !fit ==> Union(I) == analyzed;
+            assert fit ==> Union(I) == analyzed + multiset{currElement};
+            assert !fit && 0 <= i < |bins|;
+            assert !fit ==> isEnvasado(analyzed, E, I);
+            assert !fit ==> forall i: nat | 0 <= i < |bins| :: GSumNat(bins[i]) + currElement > E;
+            assume false;*/
             I, bins, capacity, fit, i := bodyLoop(A, E, i, bins, capacity, I, iterateMultiset, analyzed, fit, currElement);
+            //assume allMoreThanHalfFull(E, I) || oneLessThanHalfFull(E, I);
         } 
+        assume false;
         //If no fit was found we must create another bin
         if !fit {
             //Proof for invariants
@@ -261,21 +609,30 @@ ensures isKAproximatedBinPacking(A, E, I, 2)
             PartialSolutionIsAnalyzedNotFit(bins, bins', I, I', currElement, analyzed);
             //Proof for invariant isEnvasado(analyzed, E, I)
             EnvasadoIfNotFit(I, I', currElement, analyzed, analyzed + multiset{currElement}, E);
+            //Proof for allMoreThanHalfFull(E, I) || oneLessThanHalfFull(E, I)
+            assert I' == I + multiset{multiset{currElement}}; 
+            assert currElement <= E;
+            assert allMoreThanHalfFull(E, I') || oneLessThanHalfFull(E, I');
+            assume false;
+            assert forall i: multiset<nat> | i in I :: GSumNat(i) + currElement > E;
+            assume forall i: multiset<nat> | i in I :: GSumNat(i) + currElement > E;
+            AtMostOneLessThanHalfFullNotFIt(I, I', currElement, analyzed, analyzed + multiset{currElement}, E);
 
             bins := bins + [multiset{currElement}];
             capacity := capacity + [currElement];
             I := I + multiset{multiset{currElement}};
             //assert forall i: nat | 0 <= i < |bins| - 1 :: GSumNat(bins[i]) == capacity[i] && capacity[i] <= E;
-        }
+        }   
         partitionMaintained(A, iterateMultiset, iterateMultiset - multiset{currElement}, analyzed, analyzed + multiset{currElement}, currElement);
 
         iterateMultiset := iterateMultiset - multiset{currElement};
         analyzed := analyzed + multiset{currElement};
-        assume isEnvasado(analyzed, E, I);
+        assume false;
     }
     assume false;
     assert analyzed == A;
     assert isEnvasado(A, E, I);
-    assert allMoreThanHalfFull(E, I) || oneLessThanHalfFull(E, I);
+    assume allMoreThanHalfFull(E, I) || oneLessThanHalfFull(E, I);
     atMostOneLessThanHalfImplies2Aproximated(A, E, I);
 }
+*/
